---
title: "Chapter 1: Setting the Scene"
editor:
    render-on-save: true
---

<details>
<summary>Example 1.2</summary>
## Example 1.2

### PDE and Initial Condition

The problem is:
$$u_t + x u_x = 0, \quad x \in \mathbb{R}, t > 0,$$
$$u(x, 0) = \phi(x).$$

### Method of Characteristics
The characteristic ODE:
$$
\frac{d}{dx}u\left(x, t\right) = u_t + u_x\frac{dx}{dt}
$$
$$\frac{dx}{dt} = x, \quad x(0) = x_0.$$
Solving:
$$x(t) = x_0 e^t,$$
$$x_0 = x e^{-t}.$$

### Solution Along Characteristics
Along each characteristic:
$$
u(x(t), t) = \phi(x_0) = \phi(x e^{-t}).
$$
Thus:
$$
u(x,t) = \phi(x e^{-t}).
$$

### Verification of Solution
Using the chain rule:
$$
u(x,t) = \phi(f(x,t)), \quad f(x,t) = x e^{-t}.
$$
$$
u_x = \phi'(f(x,t)) e^{-t}, \quad u_t = \phi'(f(x,t)) (-x e^{-t}).
$$
Substituting into the PDE:
$$
u_t + x u_x = \phi'(f(x,t)) (-x e^{-t}) + x \phi'(f(x,t)) e^{-t} = 0.
$$

### Interpretation
- $\phi$ stays constant along characteristics.
- Characteristics spread out over time ($x(t) = x_0 e^t$).
- Solution “stretches” initial data along characteristics.
</details>
