---
title: "Exercise 1.11"
editor:
    render-on-save: true
---

Let $I$ denote the integral

$$
I = \int^\infty_{-\infty} e^{-x^2} dx.
$$ {#eq-I}

# a)

## Problem

Explain why

$$
I^2 = \int^\infty_{-\infty}\int^\infty_{-\infty} e^{-\left(x^2+y^2\right)} dx dy.
$$

## Solution

Since @eq-I is integrated over one variable, squaring $I$ yields

$$
I^2 = II = \left(\int^\infty_{-\infty}e^{-x}dx\right)\left(\int^\infty_{-\infty}e^{-y}dy\right)
$$

The product of the integrals can be combined such that

$$
I^2 = \int^\infty_{-\infty}\int^\infty_{-\infty} e^{-\left(x^2 + y^2\right)} dx dy
$$ {#eq-I2}

# b)

## Problem

Use polar coordinates to show that $I = \sqrt{\pi}$.

## Solution

The following identities will be used to change @eq-I2 to polar coordinates.

$$
r^2 = x^2 + y^2
$$

$$
dx dy = r dr d\theta
$$

Writing the integral @eq-I2 in terms of polar coordinates yields

$$
I^2 = \int^{2\pi}_{0}\int^\infty_0 e^{-r^2} r dr d\theta
$$

The bounds of the integrals were changed to reflect the bounds of the spaces of
the variables $\theta$ and $r$.

Carrying out the inner integral for $r$:

$$
\int^\infty_0 e^{-r^2} r dr =
-\frac{1}{2}\left[\lim_{r \rightarrow \infty} e^{-r^2} - e^0\right] =
\frac{1}{2}
$$

Carrying out the integral for $\theta$:

$$
\int^{2\pi}_0 \frac{1}{2} d\theta = \pi
$$

Therefore

$$
I^2 = \pi
$$

and

$$
I = \sqrt{\pi}
$$
